src/rel_hoare.lean
@@ -1,0 +1,26 @@
+import parlang
+
+namespace parlang
+
+variables {σ : Type} {ι : Type} {τ : ι → Type} [decidable_eq ι]
+
+def rel_hoare (P : memory τ → memory τ → Prop) (k₁ : kernel σ τ) (k₂ : kernel σ τ) (Q : memory τ → memory τ → Prop) :=
+∀ (n) s u (ac : vector bool n) m m' o o', P m m'  → exec_memory k₁ ac s m o → exec_memory k₂ ac u m' o' → Q o o'
+
+notation `{* ` P : 1 ` *} ` k₁ : 1 ` ~ ` k₂ : 1 ` {* ` Q : 1 ` *}` := rel_hoare P k₁ k₂ Q
+
+namespace rel_hoare
+
+lemma seq {P Q R} {k₁ k₁' k₂ k₂' : kernel σ τ} : {* P *} k₁ ~ k₁' {* Q *} → {* Q *} k₂ ~ k₂' {* R *} → {* P *} (k₁ ;; k₂) ~ (k₁' ;; k₂') {* R *} := begin
+    intros h₁ h₂ n s u ac m m' o o' hp hseq₁ hseq₂,
+    cases hseq₁,
+    cases hseq₂,
+    cases hseq₁_hk,
+    cases hseq₂_hk,
+    unfold rel_hoare at h₁ h₂,
+    apply h₂ n _ _ _ _ _ _ _ _ _ hseq₁_hk_a_1 hseq₂_hk_a_1,
+end
+
+end rel_hoare
+
+end parlang
